some progress on global wf

Core/Infer/Global.lean
@@ -11,10 +11,16 @@ def GlobalEnv.wf_globals : GlobalEnv -> Option Unit
 | .nil => return ()
 | .cons (.data (n := n) x k ctors) G => do
   wf_globals G
-  if (lookup x G).isNone then
-  let mctors' : Fun.Vec (Option Unit) n :=
-    λ i => spine_kinding (.data (n := 0) x k #𝓋[] :: G) (.data .cls) (ctors[i].fst) (ctors[i].snd)
-  let _ <- mctors'.to.seq
+  if (lookup x G).isNone && Vec.unique_elems (ctors.map (·.1)) then
+    let mctors' : Vec (Option Unit) n := ctors.map (λ (c : String × SpineTy) =>
+        spine_kinding (List.cons (.data (n := 0) x k #𝓋[]) G) (.data .cls) (c.1) (c.2))
+    let _ <- mctors'.seq
+    let mctors'' : Vec (Option Unit) n := ctors.map (λ c => if c.1 != x then some () else none)
+    let _ <- mctors''.seq
+    let mctors'' : Vec (Option Unit) n := ctors.map (λ (c : String × SpineTy) =>
+        if (lookup c.1 G).isNone then some () else none)
+    let _ <- mctors''.seq
+  else none
 | .cons (.openm x spTy) G => do
   wf_globals G
   if (lookup x G).isNone
@@ -35,10 +41,10 @@ def GlobalEnv.wf_globals : GlobalEnv -> Option Unit
   wf_globals G
   let e := lookup x G
   match e with
-  | some (.openm _ ⟨_, Ks, m, Ts, R⟩) => do
+  | some (.openm _ ⟨n, Ks, m, Ts, R⟩) => do
       let Γ <- pattern_binders G Ks.to_list m Ts p
       let T <- t.infer_type G Ks.to_list Γ
-      if T == R then return () else none
+      if T == R && p.length == m then return () else none
   | _ => none
 
 | .cons (.odata x _) G => do
@@ -46,11 +52,47 @@ def GlobalEnv.wf_globals : GlobalEnv -> Option Unit
   if (lookup x G).isNone
   then return () else none
 
+-- def OpenExhaustive (G : List Global) : Prop :=
+--   ∀ {x na nb} {τ : Subst Ty} {As Ks : Vec _ na} {Ts Ts' : Vec _ nb} {Δ R q},
+--   lookup x G = some (.openm x ⟨na, Ks, nb, Ts, R⟩) ->
+--   (∀ (i : Fin na), G&Δ ⊢ As[i] : Ks[i]) ->
+--   Sequ.append_vec (Vec.map su As) +0 = τ ->
+--   Vec.map (·[τ]) Ts = Ts' ->
+--   Query G .opn q Ts' ->
+--   ∃ (i : Nat), ∃ b p, G[i]? = some (.inst x p b) ∧ Query.Match q p
 
-def GlobalEnv.check_open_exhaustive : GlobalEnv -> Option Unit
-| _ => none
+def GlobalEnv.get_openm : GlobalEnv -> GlobalEnv :=
+  List.filter (λ x =>
+    match x with
+    | .openm _ _ => true
+    | _ => false)
 
--- For each method,
+def List.enumerate (l : List α) : List (Nat × α) :=
+  let t := List.foldl (λ (i, acc) x => (i + 1, acc ++ [(i, x)])) (0, .nil) l
+  t.snd
+
+
+def GlobalEnv.check_insts (G : GlobalEnv) : Global -> Option Unit
+| .openm x ⟨na, Ks, nb, Ts, R⟩ => do
+
+  let G := List.enumerate G
+
+  -- get all the instances of this method
+  let ιs := G.filter (λ e => match e with
+                             | (_, .inst y _ _) => y == x
+                             | _ => false )
+
+
+
+
+  return ()
+| _ => return ()
+
+
+def GlobalEnv.check_open_exhaustive (G : GlobalEnv) : Option Unit := do
+ let _ <- List.mapM (GlobalEnv.check_insts G) G
+
+-- For each open method,
 -- collect the instances of the method
 -- collect the patterns for each instance
 -- check that the patterns together are exhaustive
