Core/Infer/GlobalSound.lean
@@ -4,6 +4,9 @@ import Core.Infer.Global
 
 import Core.Global
 
+import Core.Vec
+
+open Lilac
 
 namespace Core
 
@@ -16,26 +19,44 @@ fun_induction GlobalEnv.wf_globals <;> simp at *
 case _ =>  -- empty
   apply ListGlobalWf.nil
 
-case _ ih => -- ctors
+case _ n x k ctors G ih => -- ctors
   rw[Option.bind_eq_some_iff] at h; rcases h with ⟨h1, h2, h⟩
-  simp at h
+  simp at h; rcases h with ⟨h3, h⟩
+  rw[Option.bind_eq_some_iff] at h; rcases h with ⟨h4, h5, h⟩
+  rw[Option.bind_eq_some_iff] at h; rcases h with ⟨h6, h7, h⟩
+  rw[Option.bind_eq_some_iff] at h; rcases h with ⟨h8, h9, h⟩
+  replace h5 := Vec.map_seq_sound _ h5
+  replace h7 := Vec.map_seq_sound _ h7
+  replace h9 := Vec.map_seq_sound _ h9
+  replace h4 := Vec.units h4;
+  rcases h3 with ⟨h3a, h3b⟩
   apply ListGlobalWf.cons
-  · sorry
+  · apply GlobalWf.data (G := G) (n := n) (K := k) (x := x) (ctors := ctors)
+    · intro i y T h
+      apply And.intro
+      · replace h5 := h5 i; rw[h] at h5; simp at h5; apply spine_kinding_sound h5
+      · apply And.intro
+        · replace h7 := h7 i; rw[h] at h7; simp at h7; simp; intro f; apply h7 (Eq.symm f)
+        · replace h9 := h9 i; rw[h] at h9; simp at h9; apply h9
+    replace h3b := Vec.unique_elems_sound h3b; simp at h3b; apply h3b
+    apply h3a
   · apply ih h2
 
 case _ ih =>  -- openm
   rw[Option.bind_eq_some_iff] at h; rcases h with ⟨h1, h2, h⟩
-  simp at h
+  simp at h;  rcases h with ⟨h3, h⟩
+  replace h := spine_kinding_sound h
+  replace ih := ih h2
   apply ListGlobalWf.cons
-  · sorry
-  · apply ih h2
+  · apply GlobalWf.openm h h3
+  · apply ih
 
 case _ ih =>  -- octor
   rw[Option.bind_eq_some_iff] at h; rcases h with ⟨h1, h2, h⟩
   simp at h; rcases h with ⟨e, h⟩
   apply ListGlobalWf.cons
   · apply GlobalWf.octor
-    sorry
+    apply spine_kinding_sound h
     apply e
   · apply ih h2
 
@@ -53,15 +74,29 @@ case _ ih => -- defn
     · apply h
   · apply ih h2
 
-case _ ih => -- inst
+case _ m _ p t G ih => -- inst
   rw[Option.bind_eq_some_iff] at h; rcases h with ⟨h1, h2, h⟩
   split at h
-  · rw[Option.bind_eq_some_iff] at h; rcases h with ⟨h3, h4, h⟩
-    rw[Option.bind_eq_some_iff] at h; rcases h with ⟨h5, h6, h⟩
-    simp at h
+  case _ x n Ks _ Ts R lk =>
+    rw[Option.bind_eq_some_iff] at h; rcases h with ⟨Γ, h4, h⟩
+    rw[Option.bind_eq_some_iff] at h; rcases h with ⟨R, h6, h⟩
+    simp at h; rcases h with ⟨e1, e2⟩; subst e1; subst e2;
+    simp [Vec.length] at *
+    replace ih := ih h2
+    replace h6 := infer_type_sound ih h6
+    have lem := lookup_name_eq lk; simp [Entry.name] at lem; subst lem
     apply ListGlobalWf.cons
-    · sorry
-    · apply ih h2
+    -- · apply GlobalWf.inst (G := G) (Δ := Ks.to_list) (x := x) (n := n) (m := m) (p := p) (t := t)
+    --   apply lk
+    --   sorry
+    --   sorry
+    --   sorry
+    --   sorry
+    --   sorry
+    --   sorry
+      sorry
+
+    · apply ih
   · cases h
 
 case _ ih => -- odata
@@ -75,6 +110,15 @@ case _ ih => -- odata
 
 theorem open_exhaustive_sound {G : GlobalEnv} :
   G.check_open_exhaustive = some () ->
-  OpenExhaustive G := by sorry
+  OpenExhaustive G
+:= by
+intro h
+unfold OpenExhaustive
+intro x na nb τ As Ks Ts Ts' Δ R q lk wk σ h1 h2
+
+unfold GlobalEnv.check_open_exhaustive at h; simp at h
+rw[Option.bind_eq_some_iff] at h; rcases h with ⟨n, h, e⟩; cases e
+sorry
+
 
 end Core
